\documentclass[12pt]{article}
\usepackage{amsmath}
\usepackage{amssymb}
\usepackage{geometry}
\geometry{a4paper, margin=1in}

\title{Homework 1 - Quantum Algorithms}
\author{Son Nguyen \\
I pledge my honor that I have abided by the Stevens Honor System.}
\date{\today}

\begin{document}

\maketitle

\section*{Problem 1.1}
For \(\bar{u}, \bar{v} \in \mathbb{C}^n\) show that the following holds:
\[ \langle u, v \rangle = \frac{1}{4}(||u+v||^2 - ||u-v||^2 - i||u+iv||^2 + i||u-iv||^2)\]
We have: 
\begin{align*}
    ||u+v||^2 &= \langle u+v, u+v \rangle = \langle u, u \rangle + \langle u, v \rangle + \langle v, u \rangle + \langle v, v \rangle \\
    ||u-v||^2 &= \langle u-v, u-v \rangle = \langle u, u \rangle - \langle u, v \rangle - \langle v, u \rangle + \langle v, v \rangle \\
    ||u+iv||^2 &= \langle u+iv, u+iv \rangle = \langle u, u \rangle + \langle u, iv \rangle + \langle iv, u \rangle + \langle iv, iv \rangle \\
    ||u-iv||^2 &= \langle u-iv, u-iv \rangle = \langle u, u \rangle - \langle u, iv \rangle - \langle iv, u \rangle + \langle iv, iv \rangle
\end{align*}
Substitute these into the equation, we have right-hand side equal to:
\begin{align*}
    &= \frac{1}{4} \left[2\left(\langle u, v \rangle + \langle v, u\rangle\right) - 2i \left(\langle u, iv\rangle + \langle iv, u\rangle\right)\right] \\
    &= \frac{1}{4} \left(2 \langle u, v \rangle + 2\langle v, u\rangle - 2\underbrace{i \cdot i}_{-1} \langle u, v\rangle - 2 \underbrace{i \cdot \bar{i}}_{1} \langle v, u\rangle\right) \\
    &= \frac{1}{4} \left(2 \langle u, v \rangle + 2\langle v, u\rangle + 2 \langle u, v\rangle - 2 \langle v, u\rangle\right) \\
    &= \frac{1}{4} \left(4 \langle u, v \rangle\right) = \langle u, v \rangle
\end{align*}
\section*{Problem 1.2}
Let \(\bar{u} = (i, 1+i)^T\) and \(\bar{v} = (2, 1-i)^T\)
\begin{enumerate}
    \item Compute \(\langle \bar{u}, \bar{v} \rangle\)
    We have the vector:
    \[\bar{u} = \begin{bmatrix}
        i \\
        1+i
    \end{bmatrix},
    \bar{v} = \begin{bmatrix}
        2 \\
        1-i
    \end{bmatrix}
    \]
    \begin{align*}
        \langle \bar{u}, \bar{v} \rangle &= \langle (i, 1+i)^T, (2, 1-i)^T \rangle \\
        \bar{u}^\dagger \cdot \bar{v} &= 
        \begin{bmatrix}
            -i & 1-i    
        \end{bmatrix}
        \cdot 
        \begin{bmatrix}
            2 \\
            1-i
        \end{bmatrix}\\
        &= -2i + 1^2 -2i + ii = -4i 
    \end{align*}
    \item Compute \(||\bar{u}||\)
    \begin{align*}
        ||\bar{u}|| &= \sqrt{\langle \bar{u}, \bar{u} \rangle} \\
        &= \sqrt{\bar{u}^\dagger \cdot \bar{u}} \\
        &= \sqrt{\begin{bmatrix}
            -i & 1-i
        \end{bmatrix}
        \cdot
        \begin{bmatrix}
            i \\
            1+i
        \end{bmatrix}} \\
        &= \sqrt{-i \cdot i + (1-i)(1+i)} \\
        &= \sqrt{1 + 2} = \sqrt{3}
    \end{align*}
    \item Express \(\frac{1}{2-i}\) in the form \(a+bi\) with \(a, b \in \mathbb{R}\)
    \begin{align*}
        \frac{1}{2-i} &= \frac{1}{2-i} \cdot \frac{2+i}{2+i} \\
        &= \frac{2+i}{5} = \frac{2}{5} + \frac{1}{5}i
    \end{align*}
\end{enumerate}
\section*{Problem 1.3}
Prove that a composition of linear transformations \(\phi, \psi: V \rightarrow V\) is linear.
\\
Let the transformation \(\phi\) be defined as \(\phi, \psi: V \rightarrow V\). Let \(v,u \in V\) and \(\alpha, \beta \in \mathbb{C}\),
the composition of \(\phi\) and \(\psi\) is defined as \(\psi \circ \phi: V \rightarrow U\):
\[(\psi \circ \phi)(\alpha v+ \beta u) = \psi(\phi(\alpha v+ \beta u))\]
Since \(\phi\) is linear, we have:
\[\phi(\alpha v+ \beta u) = \phi(\alpha u) + \phi(\beta v) = \alpha \phi(u) + \beta \phi(u)\]
Plug that back into the equation, we have:
\[ \psi(\phi(\alpha v+ \beta u))=\psi(\alpha \phi(u) + \beta \phi(u))\]
Since \(\psi\) is linear, we have:
\[\psi(\alpha \phi(u) + \beta \phi(u)) = \psi(\alpha \phi(u)) + \psi(\beta \phi(v)) = \alpha (\psi \circ \phi)(u) + \beta (\psi \circ \phi)(v)\]
Therefore, the composition of linear transformations \(\phi\) and \(\psi\) is linear.
\begin{align*}
    (\psi \circ \phi)(\alpha v+ \beta u) &= \alpha(\psi \circ \phi)(u) + \beta(\psi \circ \phi)(v)
\end{align*}
\section*{Problem 1.4}
\begin{align*}
    ||1 - e^{2ix}||^2 &= (1 - e^{2ix}) \cdot (\overline{1 - e^{2ix}}) \\
    &= [1 - (\cos(2x) + i\sin(2x))] \cdot [\overline{1 - (\cos(2x) + i\sin(2x))}] \\
    &= [1 - \cos(2x) - i\sin(2x)] \cdot [1 - \cos(2x) + i\sin(2x)] \\
    &= 1 - \cos(2x) + i\sin(2x) - \cos(2x) + \cos^2(2x) - i\sin(2x)\cos(2x) \\
    & \quad - i\sin(2x) + i\sin(2x)\cos(2x) + \sin^2(2x) \\
    &= 1 - 2\cos(2x) + \underbrace{\cos^2(2x) + \sin^2(2x)}_{1}\\
    &= 2 - 2\cos(2x) \\
    &= 2(1 - \cos(2x)) = 2 \cdot 2\sin^2(x) = 4\sin^2(x)
\end{align*}
\end{document}